Some example implications to try to prove with the new tactics

examples/BabySep.v
@@ -24,3 +24,59 @@ Theorem readOk : moduleOk read.
   sepRead.
   reflexivity.
 Qed.
+
+
+(** * Dirt-simple test cases for implication automation *)
+
+Theorem ptsto_refl : forall a v,
+  a ==> v ===> a ==> v.
+Admitted.
+
+Theorem ptsto_comm : forall a1 v1 a2 v2,
+  a1 ==> v1 * a2 ==> v2 ===> a2 ==> v2 * a1 ==> v1.
+Admitted.
+
+
+(** * Linked list ADT *)
+
+Module Type LINKED_LIST.
+  Parameter llist : list W -> W -> HProp.
+
+  Axiom llist_nil_fwd : forall ls a, a = 0
+    -> llist ls a ===> [| ls = nil |].
+
+  Axiom llist_nil_bwd : forall ls a, a = 0
+    -> [| ls = nil |] ===> llist ls a.
+
+  Axiom llist_cons_fwd : forall ls a, a <> $0
+    -> llist ls a ===> Ex x, Ex ls', Ex p, [| ls = x :: ls' |] * a ==> x * (a ^+ $1) ==> p * llist ls' p.
+
+  Axiom llist_cons_bwd : forall ls a, a <> $0
+    -> (Ex x, Ex ls', Ex p, [| ls = x :: ls' |] * a ==> x * (a ^+ $1) ==> p * llist ls' p) ===> llist ls a.
+End LINKED_LIST.
+
+Module LinkedList : LINKED_LIST.
+  Open Scope Sep_scope.
+
+  Fixpoint llist (ls : list W) (a : W) : HProp :=
+    match ls with
+      | nil => [| a = 0 |]
+      | x :: ls' => Ex p, a ==> x * (a ^+ $1) ==> p * llist ls' p
+    end.
+
+  Theorem llist_nil_fwd : forall ls a, a = 0
+    -> llist ls a ===> [| ls = nil |].
+  Admitted.
+
+  Theorem llist_nil_bwd : forall ls a, a = 0
+    -> [| ls = nil |] ===> llist ls a.
+  Admitted.
+
+  Theorem llist_cons_fwd : forall ls a, a <> $0
+    -> llist ls a ===> Ex x, Ex ls', Ex p, [| ls = x :: ls' |] * a ==> x * (a ^+ $1) ==> p * llist ls' p.
+  Admitted.
+
+  Theorem llist_cons_bwd : forall ls a, a <> $0
+    -> (Ex x, Ex ls', Ex p, [| ls = x :: ls' |] * a ==> x * (a ^+ $1) ==> p * llist ls' p) ===> llist ls a.
+  Admitted.
+End LinkedList.
